TLSConstants goes through

src/tls/TLSConstants.fst
@@ -1065,304 +1065,304 @@ let namedGroupsBytes groups =
   admit(); //TODO
   vlbytes 2 b
 
-(* //val parseNamedGroups: pinverse_t namedGroupsBytes *)
-(* let parseNamedGroups b = *)
-(*   let rec (aux: b:bytes -> list namedGroup -> Tot (Result (list namedGroup)) (decreases (length b))) = fun b groups -> *)
-(*     if length b > 0 then *)
-(*       if length b >= 2 then *)
-(* 	let (ng, bytes) = split b 2 in *)
-(* 	match parseNamedGroup ng with *)
-(* 	| Correct(ng) -> aux bytes (ng::groups) *)
-(* 	| Error(z) -> Error(z) *)
-(*       else Error (AD_decode_error, perror __SOURCE_FILE__ __LINE__ "") *)
-(*     else Correct(groups) in *)
-(*   match vlparse 2 b with *)
-(*   | Correct(b) -> aux b [] *)
-(*   | Error(z) -> Error(AD_decode_error, perror __SOURCE_FILE__ __LINE__ "Failed to parse named groups") *)
+//val parseNamedGroups: pinverse_t namedGroupsBytes
+let parseNamedGroups b =
+  let rec (aux: b:bytes -> list namedGroup -> Tot (Result (list namedGroup)) (decreases (length b))) = fun b groups ->
+    if length b > 0 then
+      if length b >= 2 then
+	let (ng, bytes) = split b 2 in
+	match parseNamedGroup ng with
+	| Correct(ng) -> aux bytes (ng::groups)
+	| Error(z) -> Error(z)
+      else Error (AD_decode_error, perror __SOURCE_FILE__ __LINE__ "")
+    else Correct(groups) in
+  match vlparse 2 b with
+  | Correct(b) -> aux b []
+  | Error(z) -> Error(AD_decode_error, perror __SOURCE_FILE__ __LINE__ "Failed to parse named groups")
 
 
-(* (\* TODO : precise configurationId type *\) *)
-(* type configurationId = b:bytes{not (equalBytes b empty_bytes) /\ length b < 65536} *)
+(* TODO : precise configurationId type *)
+type configurationId = b:bytes{not (equalBytes b empty_bytes) /\ length b < 65536}
 
-(* val configurationIdBytes: configurationId -> Tot bytes *)
-(* let configurationIdBytes cid = *)
-(*   lemma_repr_bytes_values (length cid); *)
-(*   vlbytes 2 cid *)
+val configurationIdBytes: configurationId -> Tot bytes
+let configurationIdBytes cid =
+  lemma_repr_bytes_values (length cid);
+  vlbytes 2 cid
 
-(* //val parseConfigurationId: pinverse_t configurationIdBytes *)
-(* let parseConfigurationId b = *)
-(*   vlparse 2 b *)
+//val parseConfigurationId: pinverse_t configurationIdBytes
+let parseConfigurationId b =
+  vlparse 2 b
 
-(* type uint32 = b:lbytes 4 *)
+type uint32 = b:lbytes 4
 
-(* val uint32Bytes: uint32 -> Tot (lbytes 4) *)
-(* let uint32Bytes u = u *)
+val uint32Bytes: uint32 -> Tot (lbytes 4)
+let uint32Bytes u = u
 
-(* val parseUint32: pinverse_t uint32Bytes *)
-(* let parseUint32 b = *)
-(*   if length b = 4 then Correct(b) *)
-(*   else Error (AD_decode_error, perror __SOURCE_FILE__ __LINE__ "") *)
+val parseUint32: pinverse_t uint32Bytes
+let parseUint32 b =
+  if length b = 4 then Correct(b)
+  else Error (AD_decode_error, perror __SOURCE_FILE__ __LINE__ "")
 
-(* type earlyDataType = *)
-(*   | ClientAuthentication *)
-(*   | EarlyData *)
-(*   | ClientAuthenticationAndData *)
+type earlyDataType =
+  | ClientAuthentication
+  | EarlyData
+  | ClientAuthenticationAndData
 
-(* val earlyDataTypeBytes : earlyDataType -> Tot (lbytes 1) *)
-(* let earlyDataTypeBytes edt = *)
-(*   match edt with *)
-(*   | ClientAuthentication          -> abyte 1uy *)
-(*   | EarlyData                     -> abyte 2uy *)
-(*   | ClientAuthenticationAndData   -> abyte 3uy *)
+val earlyDataTypeBytes : earlyDataType -> Tot (lbytes 1)
+let earlyDataTypeBytes edt =
+  match edt with
+  | ClientAuthentication          -> abyte 1uy
+  | EarlyData                     -> abyte 2uy
+  | ClientAuthenticationAndData   -> abyte 3uy
 
-(* val parseEarlyDataType: pinverse_t earlyDataTypeBytes *)
-(* let parseEarlyDataType b = *)
-(*     match cbyte b with *)
-(*     | (1uy) -> Correct (ClientAuthentication) *)
-(*     | (2uy) -> Correct (EarlyData) *)
-(*     | (3uy) -> Correct (ClientAuthenticationAndData) *)
-(*     | _ -> Error (AD_decode_error, perror __SOURCE_FILE__ __LINE__ "Failed to parse early data type") *)
+val parseEarlyDataType: pinverse_t earlyDataTypeBytes
+let parseEarlyDataType b =
+    match cbyte b with
+    | (1uy) -> Correct (ClientAuthentication)
+    | (2uy) -> Correct (EarlyData)
+    | (3uy) -> Correct (ClientAuthenticationAndData)
+    | _ -> Error (AD_decode_error, perror __SOURCE_FILE__ __LINE__ "Failed to parse early data type")
 
-(* // TODO : replace with more precise types when available *)
-(* type configurationExtension = *)
-(*   | UnknownConfigurationExtension: *)
-(*       typ:lbytes 2 -> payload: bytes { repr_bytes (length payload) <= 2 } -> configurationExtension *)
+// TODO : replace with more precise types when available
+type configurationExtension =
+  | UnknownConfigurationExtension:
+      typ:lbytes 2 -> payload: bytes { repr_bytes (length payload) <= 2 } -> configurationExtension
 
-(* val configurationExtensionBytes: ce:configurationExtension -> Tot bytes *)
-(* let configurationExtensionBytes ce = *)
-(*   match ce with *)
-(*   | UnknownConfigurationExtension typ payload -> typ @| vlbytes 2 payload *)
+val configurationExtensionBytes: ce:configurationExtension -> Tot bytes
+let configurationExtensionBytes ce =
+  match ce with
+  | UnknownConfigurationExtension typ payload -> typ @| vlbytes 2 payload
 
-(* val parseConfigurationExtension: pinverse_t configurationExtensionBytes *)
-(* let parseConfigurationExtension b = *)
-(*   if length b >= 4 then *)
-(*   ( let (typ, payload) = split b 2 in *)
-(*     match vlparse 2 payload with *)
-(*     | Correct (payload) -> Correct (UnknownConfigurationExtension typ payload) *)
-(*     | Error(z) -> Error(z)) *)
-(*   else Error (AD_decode_error, perror __SOURCE_FILE__ __LINE__ "Too few bytes to parse a configuration extension") *)
+val parseConfigurationExtension: pinverse_t configurationExtensionBytes
+let parseConfigurationExtension b =
+  if length b >= 4 then
+  ( let (typ, payload) = split b 2 in
+    match vlparse 2 payload with
+    | Correct (payload) -> Correct (UnknownConfigurationExtension typ payload)
+    | Error(z) -> Error(z))
+  else Error (AD_decode_error, perror __SOURCE_FILE__ __LINE__ "Too few bytes to parse a configuration extension")
 
-(* val configurationExtensionsBytes: list configurationExtension -> Tot bytes *)
-(* let configurationExtensionsBytes ce = *)
-(*   let b = (List.Tot.fold_left (fun bytes x -> bytes @| configurationExtensionBytes x) empty_bytes ce) in *)
-(*   admit(); //TODO *)
-(*   vlbytes 2 b *)
-
-
-(* val parseConfigurationExtensions: pinverse_t configurationExtensionsBytes *)
-(* let parseConfigurationExtensions b = *)
-(*   let rec (aux: b:bytes -> list configurationExtension -> Tot (Result (list configurationExtension)) (decreases (length b))) = *)
-(*     fun b exts -> *)
-(*     if length b > 0 then *)
-(*       if length b >= 4 then *)
-(* 	let typ, len, data = split2 b 2 2 in *)
-(* 	let len = int_of_bytes len in *)
-(* 	if length b >= 4 + len then *)
-(* 	  let ext, bytes = split b len in *)
-(* 	  match parseConfigurationExtension ext with *)
-(* 	  | Correct(ext') -> aux bytes (ext'::exts) *)
-(* 	  | Error(z) -> Error(z) *)
-(* 	else Error(AD_decode_error, perror __SOURCE_FILE__ __LINE__ "Failed to parse configuration extension length") *)
-(*       else Error(AD_decode_error, perror __SOURCE_FILE__ __LINE__ "Configuration extension length should be at least 4") *)
-(*     else Correct(exts) in *)
-(*   if length b >= 2 then *)
-(*   match vlparse 2 b with *)
-(*   | Correct (b) ->  aux b [] *)
-(*   | Error(z) -> Error(AD_decode_error, perror __SOURCE_FILE__ __LINE__ "Failed to parse configuration extension") *)
-(*   else Error(AD_decode_error, perror __SOURCE_FILE__ __LINE__ "Failed to parse configuration extension") *)
+val configurationExtensionsBytes: list configurationExtension -> Tot bytes
+let configurationExtensionsBytes ce =
+  let b = (List.Tot.fold_left (fun bytes x -> bytes @| configurationExtensionBytes x) empty_bytes ce) in
+  admit(); //TODO
+  vlbytes 2 b
 
 
-(* val sigHashAlgBytes: sigHashAlg -> Tot (lbytes 2) *)
-(* let sigHashAlgBytes sha = *)
-(*   let sign = sigAlgBytes (fst sha) in *)
-(*   admit(); // FIXME *)
-(*   let hash = hashAlgBytes (snd sha) in *)
-(*   hash @| sign *)
+val parseConfigurationExtensions: pinverse_t configurationExtensionsBytes
+let parseConfigurationExtensions b =
+  let rec (aux: b:bytes -> list configurationExtension -> Tot (Result (list configurationExtension)) (decreases (length b))) =
+    fun b exts ->
+    if length b > 0 then
+      if length b >= 4 then
+	let typ, len, data = split2 b 2 2 in
+	let len = int_of_bytes len in
+	if length b >= 4 + len then
+	  let ext, bytes = split b len in
+	  match parseConfigurationExtension ext with
+	  | Correct(ext') -> aux bytes (ext'::exts)
+	  | Error(z) -> Error(z)
+	else Error(AD_decode_error, perror __SOURCE_FILE__ __LINE__ "Failed to parse configuration extension length")
+      else Error(AD_decode_error, perror __SOURCE_FILE__ __LINE__ "Configuration extension length should be at least 4")
+    else Correct(exts) in
+  if length b >= 2 then
+  match vlparse 2 b with
+  | Correct (b) ->  aux b []
+  | Error(z) -> Error(AD_decode_error, perror __SOURCE_FILE__ __LINE__ "Failed to parse configuration extension")
+  else Error(AD_decode_error, perror __SOURCE_FILE__ __LINE__ "Failed to parse configuration extension")
 
-(* val parseSigHashAlg: pinverse_t sigHashAlgBytes *)
-(* let parseSigHashAlg b = *)
-(*   if length b = 2 then *)
-(*     let (hash, sign) = split b 1 in *)
-(*     match parseSigAlg sign with *)
-(*     | Correct(sign) -> *)
-(* 	(match parseHashAlg hash with *)
-(* 	| Correct(hash) -> Correct(sign, hash) *)
-(* 	| Error(z) -> Error(z)) *)
-(*     | Error(z) -> Error(z) *)
-(*   else Error (AD_decode_error, perror __SOURCE_FILE__ __LINE__ "Remaining unparsed bytes after signature hash algorithm") *)
 
-(* val sigHashAlgsBytes: list sigHashAlg -> Tot bytes *)
-(* let sigHashAlgsBytes algs = *)
-(*   admit(); // TODO *)
-(*   vlbytes 2 (List.Tot.fold_left (fun l x -> sigHashAlgBytes x @| l) empty_bytes algs) *)
+val sigHashAlgBytes: sigHashAlg -> Tot (lbytes 2)
+let sigHashAlgBytes sha =
+  let sign = sigAlgBytes (fst sha) in
+  admit(); // FIXME
+  let hash = hashAlgBytes (snd sha) in
+  hash @| sign
 
-(* val parseSigHashAlgs: pinverse_t sigHashAlgsBytes *)
-(* let parseSigHashAlgs b = *)
-(*   let rec (aux: b:bytes -> list sigHashAlg -> Tot (Result (list sigHashAlg)) (decreases (length b))) = fun b algs -> *)
-(*     if length b > 0 then *)
-(*       if length b >= 2 then *)
-(*       let (alg, bytes) = split b 2 in *)
-(*       match parseSigHashAlg alg with *)
-(*       | Correct(sha) -> aux bytes (sha::algs) *)
-(*       | Error(z) -> Error(z) *)
-(*       else Error (AD_decode_error, perror __SOURCE_FILE__ __LINE__ "Too few bytes to parse sig hash algs") *)
-(*     else Correct(algs) in *)
-(*   match vlparse 2 b with *)
-(*   | Correct (b) -> aux b [] *)
-(*   | Error(z) -> Error(AD_decode_error, perror __SOURCE_FILE__ __LINE__ "Failed to parse sig hash algs") *)
+val parseSigHashAlg: pinverse_t sigHashAlgBytes
+let parseSigHashAlg b =
+  if length b = 2 then
+    let (hash, sign) = split b 1 in
+    match parseSigAlg sign with
+    | Correct(sign) ->
+	(match parseHashAlg hash with
+	| Correct(hash) -> Correct(sign, hash)
+	| Error(z) -> Error(z))
+    | Error(z) -> Error(z)
+  else Error (AD_decode_error, perror __SOURCE_FILE__ __LINE__ "Remaining unparsed bytes after signature hash algorithm")
 
-(* // TODO : replace "bytes" by either DH or ECDH parameters *)
-(* type keyShareEntry = namedGroup * b:bytes { repr_bytes (length b) <= 2 } *)
+val sigHashAlgsBytes: list sigHashAlg -> Tot bytes
+let sigHashAlgsBytes algs =
+  admit(); // TODO
+  vlbytes 2 (List.Tot.fold_left (fun l x -> sigHashAlgBytes x @| l) empty_bytes algs)
 
-(* val keyShareEntryBytes: keyShareEntry -> Tot bytes *)
-(* let keyShareEntryBytes (ng, bytes) = *)
-(*   let ng_bytes = namedGroupBytes ng in *)
-(*   ng_bytes @| vlbytes 2 bytes *)
+val parseSigHashAlgs: pinverse_t sigHashAlgsBytes
+let parseSigHashAlgs b =
+  let rec (aux: b:bytes -> list sigHashAlg -> Tot (Result (list sigHashAlg)) (decreases (length b))) = fun b algs ->
+    if length b > 0 then
+      if length b >= 2 then
+      let (alg, bytes) = split b 2 in
+      match parseSigHashAlg alg with
+      | Correct(sha) -> aux bytes (sha::algs)
+      | Error(z) -> Error(z)
+      else Error (AD_decode_error, perror __SOURCE_FILE__ __LINE__ "Too few bytes to parse sig hash algs")
+    else Correct(algs) in
+  match vlparse 2 b with
+  | Correct (b) -> aux b []
+  | Error(z) -> Error(AD_decode_error, perror __SOURCE_FILE__ __LINE__ "Failed to parse sig hash algs")
 
-(* val parseKeyShareEntry: pinverse_t keyShareEntryBytes *)
-(* let parseKeyShareEntry b = *)
-(*   if length b >= 2 then *)
-(*     let ng, key_exchange = split b 2 in *)
-(*     match parseNamedGroup ng with *)
-(*     | Correct(ng) -> *)
-(* 	(match vlparse 2 key_exchange with *)
-(* 	| Correct(ke) -> Correct (ng, ke) *)
-(* 	| Error(z) -> Error(AD_decode_error, perror __SOURCE_FILE__ __LINE__ "Failed to parse key share entry")) *)
-(*     | Error(z) -> Error(z) *)
-(*   else Error (AD_decode_error, perror __SOURCE_FILE__ __LINE__ "Too few bytes to parse key share entry") *)
+// TODO : replace "bytes" by either DH or ECDH parameters
+type keyShareEntry = namedGroup * b:bytes { repr_bytes (length b) <= 2 }
 
-(* val keyShareEntriesBytes: list keyShareEntry -> Tot bytes *)
-(* let keyShareEntriesBytes kses = *)
-(*   admit(); //TODO *)
-(*   vlbytes 2 (List.Tot.fold_left (fun l s -> l @| keyShareEntryBytes s) empty_bytes kses) *)
+val keyShareEntryBytes: keyShareEntry -> Tot bytes
+let keyShareEntryBytes (ng, bytes) =
+  let ng_bytes = namedGroupBytes ng in
+  ng_bytes @| vlbytes 2 bytes
 
-(* val parseKeyShareEntries: pinverse_t keyShareEntriesBytes *)
-(* let parseKeyShareEntries b = *)
-(*   let rec (aux: b:bytes -> list keyShareEntry -> Tot (Result (list keyShareEntry)) (decreases(length b))) = fun b entries -> *)
-(*     if length b > 0 then *)
-(*       if length b >= 4 then *)
-(* 	let (ng, data) = split b 2 in *)
-(* 	match vlsplit 2 data with *)
-(* 	| Correct(kex, bytes) -> *)
-(* 	    (match parseKeyShareEntry (ng @| vlbytes 2 kex) with *)
-(* 	    | Correct(entry) -> aux bytes (entry::entries) *)
-(* 	    | Error(z) -> Error(z)) *)
-(* 	| Error(z) -> Error(AD_decode_error, perror __SOURCE_FILE__ __LINE__ "Failed to parse key share entry") *)
-(*       else Error (AD_decode_error, perror __SOURCE_FILE__ __LINE__ "Too few bytes to parse key share entries") *)
-(*     else Correct(entries) in *)
-(*   match vlparse 2 b with *)
-(*   | Correct (b) ->  aux b [] *)
-(*   | Error(z) -> Error(AD_decode_error, perror __SOURCE_FILE__ __LINE__ "Failed to parse key share entries") *)
+val parseKeyShareEntry: pinverse_t keyShareEntryBytes
+let parseKeyShareEntry b =
+  if length b >= 2 then
+    let ng, key_exchange = split b 2 in
+    match parseNamedGroup ng with
+    | Correct(ng) ->
+	(match vlparse 2 key_exchange with
+	| Correct(ke) -> Correct (ng, ke)
+	| Error(z) -> Error(AD_decode_error, perror __SOURCE_FILE__ __LINE__ "Failed to parse key share entry"))
+    | Error(z) -> Error(z)
+  else Error (AD_decode_error, perror __SOURCE_FILE__ __LINE__ "Too few bytes to parse key share entry")
+
+val keyShareEntriesBytes: list keyShareEntry -> Tot bytes
+let keyShareEntriesBytes kses =
+  admit(); //TODO
+  vlbytes 2 (List.Tot.fold_left (fun l s -> l @| keyShareEntryBytes s) empty_bytes kses)
+
+val parseKeyShareEntries: pinverse_t keyShareEntriesBytes
+let parseKeyShareEntries b =
+  let rec (aux: b:bytes -> list keyShareEntry -> Tot (Result (list keyShareEntry)) (decreases(length b))) = fun b entries ->
+    if length b > 0 then
+      if length b >= 4 then
+	let (ng, data) = split b 2 in
+	match vlsplit 2 data with
+	| Correct(kex, bytes) ->
+	    (match parseKeyShareEntry (ng @| vlbytes 2 kex) with
+	    | Correct(entry) -> aux bytes (entry::entries)
+	    | Error(z) -> Error(z))
+	| Error(z) -> Error(AD_decode_error, perror __SOURCE_FILE__ __LINE__ "Failed to parse key share entry")
+      else Error (AD_decode_error, perror __SOURCE_FILE__ __LINE__ "Too few bytes to parse key share entries")
+    else Correct(entries) in
+  match vlparse 2 b with
+  | Correct (b) ->  aux b []
+  | Error(z) -> Error(AD_decode_error, perror __SOURCE_FILE__ __LINE__ "Failed to parse key share entries")
   
-(* type clientKeyShare = l:list keyShareEntry{List.Tot.length l >= 4 /\ List.Tot.length l < 65536} *)
-(* type serverKeyShare = keyShareEntry *)
+type clientKeyShare = l:list keyShareEntry{List.Tot.length l >= 4 /\ List.Tot.length l < 65536}
+type serverKeyShare = keyShareEntry
 
-(* type keyShare = *)
-(*   | ClientKeyShare of clientKeyShare *)
-(*   | ServerKeyShare of serverKeyShare *)
+type keyShare =
+  | ClientKeyShare of clientKeyShare
+  | ServerKeyShare of serverKeyShare
 
-(* val clientKeyShareBytes: clientKeyShare -> Tot bytes *)
-(* let clientKeyShareBytes cks = *)
-(*   keyShareEntriesBytes cks *)
+val clientKeyShareBytes: clientKeyShare -> Tot bytes
+let clientKeyShareBytes cks =
+  keyShareEntriesBytes cks
 
-(* //val parseClientKeyShare: pinverse_t clientKeyShareBytes *)
-(* let parseClientKeyShare b = parseKeyShareEntries b *)
+//val parseClientKeyShare: pinverse_t clientKeyShareBytes
+let parseClientKeyShare b = parseKeyShareEntries b
 
-(* val serverKeyShareBytes: serverKeyShare -> Tot bytes *)
-(* let serverKeyShareBytes sks = keyShareEntryBytes sks *)
+val serverKeyShareBytes: serverKeyShare -> Tot bytes
+let serverKeyShareBytes sks = keyShareEntryBytes sks
 
-(* val parseServerKeyShare: pinverse_t serverKeyShareBytes *)
-(* let parseServerKeyShare b = parseKeyShareEntry b *)
+val parseServerKeyShare: pinverse_t serverKeyShareBytes
+let parseServerKeyShare b = parseKeyShareEntry b
 
-(* val keyShareBytes: keyShare -> Tot bytes *)
-(* let keyShareBytes = function *)
-(*   | ClientKeyShare cks -> clientKeyShareBytes cks *)
-(*   | ServerKeyShare sks -> serverKeyShareBytes sks *)
+val keyShareBytes: keyShare -> Tot bytes
+let keyShareBytes = function
+  | ClientKeyShare cks -> clientKeyShareBytes cks
+  | ServerKeyShare sks -> serverKeyShareBytes sks
 
-(* (\* TODO: FIXME *\) *)
-(* val parseKeyShare: pinverse_t keyShareBytes *)
-(* let parseKeyShare b = *)
-(*   admit(); //FIXME *)
-(*   match parseKeyShareEntries b with *)
-(*   | Correct(kse) -> *)
-(*       (match kse with *)
-(*       | e::[] -> Correct(ServerKeyShare e) *)
-(*       | _ -> if List.Tot.length kse >= 2 && List.Tot.length kse < 65536 then Correct(ClientKeyShare (kse)) *)
-(* 	     else Error (AD_decode_error, perror __SOURCE_FILE__ __LINE__ "Wrong key share length") ) *)
-(*   | Error(z) -> Error(z) *)
+(* TODO: FIXME *)
+val parseKeyShare: pinverse_t keyShareBytes
+let parseKeyShare b =
+  admit(); //FIXME
+  match parseKeyShareEntries b with
+  | Correct(kse) ->
+      (match kse with
+      | e::[] -> Correct(ServerKeyShare e)
+      | _ -> if List.Tot.length kse >= 2 && List.Tot.length kse < 65536 then Correct(ClientKeyShare (kse))
+	     else Error (AD_decode_error, perror __SOURCE_FILE__ __LINE__ "Wrong key share length") )
+  | Error(z) -> Error(z)
 
-(* // TODO : give more precise type *)
-(* type pskIdentity = b:bytes{length b < 65536} *)
+// TODO : give more precise type
+type pskIdentity = b:bytes{length b < 65536}
 
-(* val pskIdentityBytes: pskIdentity -> Tot bytes *)
-(* let pskIdentityBytes pski = *)
-(*   lemma_repr_bytes_values (length pski); *)
-(*   vlbytes 2 (pski) *)
+val pskIdentityBytes: pskIdentity -> Tot bytes
+let pskIdentityBytes pski =
+  lemma_repr_bytes_values (length pski);
+  vlbytes 2 (pski)
 
-(* //val parsePskIdentity: pinverse_t pskIdentityBytes *)
-(* let parsePskIdentity b = vlparse 2 b *)
+//val parsePskIdentity: pinverse_t pskIdentityBytes
+let parsePskIdentity b = vlparse 2 b
 
-(* val pskIdentitiesBytes: list pskIdentity -> Tot bytes *)
-(* let pskIdentitiesBytes l = *)
-(*   admit(); // TODO *)
-(*   vlbytes 2 (List.Tot.fold_left (fun l s -> l @| pskIdentityBytes s) empty_bytes l) *)
+val pskIdentitiesBytes: list pskIdentity -> Tot bytes
+let pskIdentitiesBytes l =
+  admit(); // TODO
+  vlbytes 2 (List.Tot.fold_left (fun l s -> l @| pskIdentityBytes s) empty_bytes l)
 
-(* val parsePskIdentities: pinverse_t pskIdentitiesBytes *)
-(* let parsePskIdentities b = *)
-(*   let rec (aux: b:bytes -> list pskIdentity -> Tot (Result (list pskIdentity)) (decreases (length b))) = fun b ids -> *)
-(*     if length b > 0 then *)
-(*       if length b >= 2 then *)
-(* 	let len, data = split b 2 in *)
-(* 	let len = int_of_bytes len in *)
-(* 	if length b >= len then *)
-(* 	  let pski, bytes = split b len in *)
-(* 	  match parsePskIdentity pski with *)
-(* 	  | Correct(id) -> *)
-(*               admit(); // TODO *)
-(*               aux bytes (id::ids) *)
-(* 	  | Error(z) -> Error(z) *)
-(*         else Error(AD_decode_error, perror __SOURCE_FILE__ __LINE__ "Failed to parse psk identity length") *)
-(*       else Error(AD_decode_error, perror __SOURCE_FILE__ __LINE__ "Expected psk identity to be at least 2 bytes long") *)
-(*     else Correct(ids) in *)
-(*   match vlparse 2 b with *)
-(*   | Correct (b) -> aux b [] *)
-(*   | Error(z) -> Error(AD_decode_error, perror __SOURCE_FILE__ __LINE__ "Failed to parse psk identities") *)
+val parsePskIdentities: pinverse_t pskIdentitiesBytes
+let parsePskIdentities b =
+  let rec (aux: b:bytes -> list pskIdentity -> Tot (Result (list pskIdentity)) (decreases (length b))) = fun b ids ->
+    if length b > 0 then
+      if length b >= 2 then
+	let len, data = split b 2 in
+	let len = int_of_bytes len in
+	if length b >= len then
+	  let pski, bytes = split b len in
+	  match parsePskIdentity pski with
+	  | Correct(id) ->
+              admit(); // TODO
+              aux bytes (id::ids)
+	  | Error(z) -> Error(z)
+        else Error(AD_decode_error, perror __SOURCE_FILE__ __LINE__ "Failed to parse psk identity length")
+      else Error(AD_decode_error, perror __SOURCE_FILE__ __LINE__ "Expected psk identity to be at least 2 bytes long")
+    else Correct(ids) in
+  match vlparse 2 b with
+  | Correct (b) -> aux b []
+  | Error(z) -> Error(AD_decode_error, perror __SOURCE_FILE__ __LINE__ "Failed to parse psk identities")
 
-(* type clientPreSharedKey = l:list pskIdentity{List.Tot.length l >= 2 /\ List.Tot.length l < 65536 } *)
-(* type serverPreSharedKey = pskIdentity *)
-(* type preSharedKey = *)
-(*   | ClientPreSharedKey of clientPreSharedKey *)
-(*   | ServerPreSharedKey of serverPreSharedKey *)
+type clientPreSharedKey = l:list pskIdentity{List.Tot.length l >= 2 /\ List.Tot.length l < 65536 }
+type serverPreSharedKey = pskIdentity
+type preSharedKey =
+  | ClientPreSharedKey of clientPreSharedKey
+  | ServerPreSharedKey of serverPreSharedKey
 
-(* val clientPreSharedKeyBytes: clientPreSharedKey -> Tot bytes *)
-(* let clientPreSharedKeyBytes cpsk = pskIdentitiesBytes cpsk *)
+val clientPreSharedKeyBytes: clientPreSharedKey -> Tot bytes
+let clientPreSharedKeyBytes cpsk = pskIdentitiesBytes cpsk
 
-(* //val parseClientPreSharedKey: pinverse_t clientPreSharedKeyBytes *)
-(* let parseClientPreSharedKey b = parsePskIdentities b *)
+//val parseClientPreSharedKey: pinverse_t clientPreSharedKeyBytes
+let parseClientPreSharedKey b = parsePskIdentities b
 
-(* val serverPreSharedKeyBytes: serverPreSharedKey -> Tot bytes *)
-(* let serverPreSharedKeyBytes cpsk = pskIdentityBytes cpsk *)
+val serverPreSharedKeyBytes: serverPreSharedKey -> Tot bytes
+let serverPreSharedKeyBytes cpsk = pskIdentityBytes cpsk
 
-(* //val parseServerPreSharedKey: pinverse_t serverPreSharedKeyBytes *)
-(* let parseServerPreSharedKey b = parsePskIdentity b *)
+//val parseServerPreSharedKey: pinverse_t serverPreSharedKeyBytes
+let parseServerPreSharedKey b = parsePskIdentity b
 
-(* val preSharedKeyBytes: preSharedKey -> Tot bytes *)
-(* let preSharedKeyBytes = function *)
-(*   | ClientPreSharedKey cpsk -> clientPreSharedKeyBytes cpsk *)
-(*   | ServerPreSharedKey spsk -> serverPreSharedKeyBytes spsk *)
+val preSharedKeyBytes: preSharedKey -> Tot bytes
+let preSharedKeyBytes = function
+  | ClientPreSharedKey cpsk -> clientPreSharedKeyBytes cpsk
+  | ServerPreSharedKey spsk -> serverPreSharedKeyBytes spsk
 
-(* val parsePreSharedKey: pinverse_t preSharedKeyBytes *)
-(* let parsePreSharedKey b = *)
-(*   match vlparse 2 b with *)
-(*   | Correct(b') -> *)
-(*       (match vlparse 2 b with *)
-(*       | Correct(b'') -> // Client case *)
-(* 	(match parseClientPreSharedKey b with *)
-(* 	| Correct(psks) -> admit(); //TODO *)
-(*                           Correct(ClientPreSharedKey psks) *)
-(* 	| Error(z) -> Error(z)) *)
-(*       | Error(_) -> // Server case *)
-(* 	(match parseServerPreSharedKey b with *)
-(* 	| Correct(psk) -> Correct (ServerPreSharedKey psk) *)
-(* 	| Error(z) -> Error(z))) *)
-(*   | Error(z) -> Error(AD_decode_error, perror __SOURCE_FILE__ __LINE__ "Failed to parse pre shared key") *)
+val parsePreSharedKey: pinverse_t preSharedKeyBytes
+let parsePreSharedKey b =
+  match vlparse 2 b with
+  | Correct(b') ->
+      (match vlparse 2 b with
+      | Correct(b'') -> // Client case
+	(match parseClientPreSharedKey b with
+	| Correct(psks) -> admit(); //TODO
+                          Correct(ClientPreSharedKey psks)
+	| Error(z) -> Error(z))
+      | Error(_) -> // Server case
+	(match parseServerPreSharedKey b with
+	| Correct(psk) -> Correct (ServerPreSharedKey psk)
+	| Error(z) -> Error(z)))
+  | Error(z) -> Error(AD_decode_error, perror __SOURCE_FILE__ __LINE__ "Failed to parse pre shared key")
